A long journey towards the pushability, again

src/RqRsCorrect.v
@@ -4,6 +4,8 @@ Require Import Syntax Semantics StepM Invariant Serial.
 Require Import Reduction Commutable QuasiSeq Topology.
 Require Import RqRsTopo RqRsInv.
 
+Set Implicit Arguments.
+
 Open Scope list.
 Open Scope fmap.
 
@@ -21,6 +23,114 @@ Open Scope fmap.
  *    2) Theorem (disjointness of [hst]): [∀hst. h1 -*- hst \/ hst -*- h2]
  * 4. Theorem: [∀h1 h2. h1 -*- h2 -> MDisjoint h1 h2 -> Commutable h1 h2]
  *)
+
+Section Pushable.
+  Context {oifc: OStateIfc}.
+  Variables (dtr: DTree)
+            (sys: System oifc).
+
+  Hypothesis (Hrrs: RqRsSys dtr sys).
+
+  Variables (phst: MHistory)
+            (oidx ridx: IdxT)
+            (rins routs: list (Id Msg)).
+  Hypothesis (Hcont: ValidExtContinuousL
+                       sys phst (RlblInt oidx ridx rins routs)).
+
+  Local Definition nlbl := (RlblInt oidx ridx rins routs).
+  
+  (*   RqUpMsgs dtr oidx rins \/ *)
+  (*   (RqDownMsgs dtr oidx rins /\ *)
+  (*    SubList (rssOf hst) (subtreeInds dtr (parentOf dtr oidx))). *)
+  Definition RqRsLPush (hst: MHistory): Prop :=
+    DisjList (rssOf phst) (rssOf hst).
+
+  (*   RsUpMsgs dtr oidx rins \/ *)
+  (*   RsDownMsgs dtr oidx rins \/ *)
+  (*   (RqDownMsgs dtr oidx rins /\ *)
+  (*    DisjList (rssOf hst) (subtreeInds dtr (parentOf dtr oidx))). *)
+  Definition RqRsRPush (hst: MHistory): Prop :=
+    ~ In oidx (rssOf hst).
+
+  Lemma rqrs_previous_rpush: RqRsRPush phst.
+  Proof.
+    (** requires the [GoodIteration] invariant *)
+  Admitted.
+
+  Lemma rqrs_next_lpush: RqRsLPush [RlblInt oidx ridx rins routs].
+  Proof.
+    (** requires the [GoodIteration] invariant *)
+  Admitted.
+
+  Lemma rqrs_lpush_or_rpush:
+    forall st1,
+      Reachable (steps step_m) sys st1 ->
+      forall hsts st2,
+        Forall (AtomicEx msg_dec) hsts ->
+        steps step_m sys st1 (nlbl :: List.concat hsts ++ phst) st2 ->
+        Forall (fun hst => Discontinuous phst hst) hsts ->
+        Forall (fun hst => RqRsLPush hst \/ RqRsRPush hst) hsts.
+  Proof.
+  Admitted.
+
+  Lemma rqrs_left_right_pushable_phst:
+    forall st1,
+      Reachable (steps step_m) sys st1 ->
+      forall hsts st2,
+        Forall (AtomicEx msg_dec) hsts ->
+        steps step_m sys st1 (nlbl :: List.concat hsts ++ phst) st2 ->
+        Forall (fun hst => Discontinuous phst hst) hsts ->
+        LRPushable sys RqRsLPush RqRsRPush (hsts ++ [phst]).
+  Proof.
+  Admitted.
+
+  Lemma rqrs_left_right_pushable_nlbl:
+    forall st1,
+      Reachable (steps step_m) sys st1 ->
+      forall hsts st2,
+        Forall (AtomicEx msg_dec) hsts ->
+        steps step_m sys st1 (nlbl :: List.concat hsts ++ phst) st2 ->
+        Forall (fun hst => Discontinuous phst hst) hsts ->
+        LRPushable sys RqRsLPush RqRsRPush ([nlbl] :: hsts).
+  Proof.
+  Admitted.
+
+End Pushable.
+
+Theorem rqrs_pushable:
+  forall {oifc} (sys: System oifc) (dtr: DTree),
+    RqRsSys dtr sys ->
+    Pushable sys.
+Proof.
+  intros; red; intros.
+
+  assert (exists oidx ridx rins routs,
+             l2 = RlblInt oidx ridx rins routs) as Hnlbl.
+  { inv H0; inv H1.
+    destruct H0 as [oidx [ridx [rins [routs ?]]]]; dest; subst.
+    do 4 eexists; reflexivity.
+  }
+  destruct Hnlbl as [oidx [ridx [rins [routs ?]]]]; subst.
+  
+  exists (RqRsLPush hst1), (RqRsRPush oidx).
+  repeat split.
+  - eauto using rqrs_previous_rpush.
+  - eauto using rqrs_next_lpush.
+  - eauto using rqrs_lpush_or_rpush.
+  - eauto using rqrs_left_right_pushable_phst.
+  - eauto using rqrs_left_right_pushable_nlbl.
+Qed.
+
+Corollary rqrs_serializable:
+  forall {oifc} (sys: System oifc) (dtr: DTree),
+    RqRsSys dtr sys ->
+    SerializableSys sys.
+Proof.
+  intros.
+  apply well_interleaved_serializable.
+  apply well_interleaved_push_ok.
+  eapply rqrs_pushable; eauto.
+Qed.
 
 Close Scope list.
 Close Scope fmap.
